Use Map, adjust to the new LExpr T style

Strata/DL/Lambda/Semantics.lean
@@ -13,103 +13,102 @@ import Strata.DL.Lambda.LState
 
 namespace Lambda
 
-variable {IDMeta:Type} [DecidableEq IDMeta]
+variable {T : LExprParamsT} [DecidableEq T.base.Metadata]
+    [DecidableEq T.base.Identifier] [DecidableEq T.base.IDMeta]
+    [Traceable LExpr.EvalProvenance T.base.Metadata]
 
 open Lambda
 
 /--
 A free variable -> expression mapping.
 -/
-abbrev FreeVarMap := Map (Identifier IDMeta) (LExpr LMonoTy IDMeta)
+abbrev Env (T:LExprParamsT) := T.base.Identifier → Option (LExpr T)
 
-@[reducible]
-def Scopes.toFreeVarMap (s:Scopes IDMeta)
-    : Map (Identifier IDMeta) (LExpr LMonoTy IDMeta) :=
-  (List.flatten s).map (fun (id,(_,e)) => (id,e))
+def Scopes.toFreeVarMap (s:Scopes T.base) : Env T.base.mono :=
+  fun t => (s.find? t).map (·.snd)
 
 /--
 A small-step semantics of LExpr.
 Currently only defined for LMonoTy, but it will be expanded to an arbitrary
-type.
+type in the future.
 The order of constructors matter because the `constructor` tactic will rely on
 it.
 This small-step definitions faithfully follows the behavior of LExpr.eval,
-except that this inductive definition may stuck early when there is no
+except that
+(1) This inductive definition may stuck early when there is no
 assignment to a free variable available.
+(2) This semantics does not describe how the metadata must change, because
+metadata must not affect evaluation semantics. Different concrete evaluators
+like LExpr.eval can use different strategy for updating metadata.
 -/
-inductive Step (F:@Factory IDMeta) (rf:FreeVarMap)
-  : LExpr LMonoTy IDMeta → LExpr LMonoTy IDMeta → Prop where
+inductive Step (F:@Factory T.base.mono.base) (rf:Env T.base.mono)
+  : LExpr T.base.mono → LExpr T.base.mono → Prop where
 -- A free variable. Stuck if fvar does not exist in FreeVarMap.
 | expand_fvar:
-  ∀ (x:Identifier IDMeta) (e:LExpr LMonoTy IDMeta),
-    rf.find? x = .some e →
-    Step F rf (.fvar x ty) e
+  ∀ (x:T.base.mono.base.Identifier) (e:LExpr T.base.mono),
+    rf x = .some e →
+    Step F rf (.fvar _ x ty) e
 
 -- Beta reduction for lambda; Call-by-value semantics.
 | beta:
-  ∀ (e1 v2:LExpr LMonoTy IDMeta),
+  ∀ (e1 v2 eres:LExpr T.base.mono),
     LExpr.isCanonicalValue F v2 →
-    Step F rf (.app (.abs ty e1) v2) (LExpr.subst v2 e1)
+    eres = LExpr.subst (fun _ => v2) e1 →
+    Step F rf (.app m1 (.abs m2 ty e1) v2) eres
 
 -- Call-by-value semantics.
 | reduce_2:
-  ∀ (v1 e2 e2':LExpr LMonoTy IDMeta),
+  ∀ (v1 e2 e2':LExpr T.base.mono),
     LExpr.isCanonicalValue F v1 →
     Step F rf e2 e2' →
-    Step F rf (.app v1 e2) (.app v1 e2')
+    Step F rf (.app m v1 e2) (.app m' v1 e2')
 
 | reduce_1:
-  ∀ (e1 e1' e2:LExpr LMonoTy IDMeta),
+  ∀ (e1 e1' e2:LExpr T.base.mono),
     Step F rf e1 e1' →
-    Step F rf (.app e1 e2) (.app e1' e2)
+    Step F rf (.app m e1 e2) (.app m' e1' e2)
 
 -- For ite x e1 e2, do not eagerly evaluate e1 and e2.
 -- For the reduction order, ite x e1 e2 is interpreted as
 -- 'ite x (λ.e1) (λ.e2)'.
 | ite_reduce_then:
-  ∀ (ethen eelse:LExpr LMonoTy IDMeta),
-    Step F rf (.ite (.const (.boolConst true)) ethen eelse) ethen
+  ∀ (ethen eelse:LExpr T.base.mono),
+    Step F rf (.ite m (.const mc (.boolConst true)) ethen eelse) ethen
 
 | ite_reduce_else:
-  ∀ (ethen eelse:LExpr LMonoTy IDMeta),
-    Step F rf (.ite (.const (.boolConst false)) ethen eelse) eelse
+  ∀ (ethen eelse:LExpr T.base.mono),
+    Step F rf (.ite m (.const mc (.boolConst false)) ethen eelse) eelse
 
 | ite_reduce_cond:
-  ∀ (econd econd' ethen eelse:LExpr LMonoTy IDMeta),
+  ∀ (econd econd' ethen eelse:LExpr T.base.mono),
     Step F rf econd econd' →
-    Step F rf (.ite econd ethen eelse) (.ite econd' ethen eelse)
+    Step F rf (.ite m econd ethen eelse) (.ite m' econd' ethen eelse)
 
 -- Equality. Reduce after both operands evaluate to values.
 | eq_reduce:
-  ∀ (e1 e2 eres:LExpr LMonoTy IDMeta)
+  ∀ (e1 e2 eres:LExpr T.base.mono)
     (H1:LExpr.isCanonicalValue F e1)
     (H2:LExpr.isCanonicalValue F e2),
-    eres = .const (.boolConst (LExpr.eql F e1 e2 H1 H2)) →
-    Step F rf (.eq e1 e2) eres
+    eres = .const mc (.boolConst (LExpr.eql F e1 e2 H1 H2)) →
+    Step F rf (.eq m e1 e2) eres
 
 | eq_reduce_lhs:
-  ∀ (e1 e1' e2:LExpr LMonoTy IDMeta),
+  ∀ (e1 e1' e2:LExpr T.base.mono),
     Step F rf e1 e1' →
-    Step F rf (.eq e1 e2) (.eq e1' e2)
+    Step F rf (.eq m e1 e2) (.eq m' e1' e2)
 
 | eq_reduce_rhs:
-  ∀ (v1 e2 e2':LExpr LMonoTy IDMeta),
+  ∀ (v1 e2 e2':LExpr T.base.mono),
     LExpr.isCanonicalValue F v1 →
     Step F rf e2 e2' →
-    Step F rf (.eq v1 e2) (.eq v1 e2')
-
--- Evaluation keeps the metadata.
-| mdata:
-  ∀ (e e':LExpr LMonoTy IDMeta) (m:Info),
-    Step F rf e e' →
-    Step F rf (.mdata m e) (.mdata m e')
+    Step F rf (.eq m v1 e2) (.eq m' v1 e2')
 
 -- Expand functions and free variables when they are evaluated.
 -- If the function body is unknown, concreteEval can be instead used. Look at
 -- the eval_fn constructor below.
 -- This is consistent with what LExpr.eval does (modulo the "inline" flag).
 | expand_fn:
-  ∀ (e callee fnbody new_body:LExpr LMonoTy IDMeta) args fn,
+  ∀ (e callee fnbody new_body:LExpr T.base.mono) args fn,
     F.callOfLFunc e = .some (callee,args,fn) →
     args.all (LExpr.isCanonicalValue F) →
     fn.body = .some fnbody →
@@ -120,16 +119,18 @@ inductive Step (F:@Factory IDMeta) (rf:FreeVarMap)
 -- If LFunc has a concrete evaluator, this can be used to 'jump' to the final
 -- result of the function.
 | eval_fn:
-  ∀ (e callee:LExpr LMonoTy IDMeta) args fn denotefn,
+  ∀ (e callee:LExpr T.base.mono) args fn denotefn,
     F.callOfLFunc e = .some (callee,args,fn) →
     args.all (LExpr.isCanonicalValue F) →
     fn.concreteEval = .some denotefn →
-    Step F rf e (denotefn (LExpr.mkApp callee args) args)
+    Step F rf e (denotefn (LExpr.mkApp m callee args) args)
 
 
+omit [DecidableEq T.base.Metadata] [DecidableEq T.base.Identifier]
+     [Traceable LExpr.EvalProvenance T.base.Metadata] in
 theorem step_const_stuck:
-  ∀ (F:@Factory IDMeta) r x e,
-  ¬ Step F r (.const x) e := by
+  ∀ (F:@Factory T.base) r x e,
+  ¬ Step F r (.const m x) e := by
   intros
   intro H
   contradiction
@@ -137,8 +138,8 @@ theorem step_const_stuck:
 /--
 Multi-step execution: reflexive transitive closure of single steps.
 -/
-inductive StepStar (F:@Factory IDMeta) (rf:@FreeVarMap IDMeta)
-  : LExpr LMonoTy IDMeta → LExpr LMonoTy IDMeta → Prop where
+inductive StepStar (F:@Factory T.base) (rf:Env T.base.mono)
+  : LExpr T.base.mono → LExpr T.base.mono → Prop where
 | refl : StepStar F rf e e
 | step : ∀ e e' e'', Step F rf e e' → StepStar F rf e' e''
         → StepStar F rf e e''
